pok

Generic_KE.ec
@@ -8,7 +8,7 @@ require (*--*) FinType.
 require import AllpairsProp.
 
 
-type ct, pt, rt, irt.
+type ct, pt, rt, irt, auxt.
 
 op d : ct distr.
 axiom duni : is_uniform d.
@@ -20,22 +20,22 @@ axiom ss c : mu1 d c = 1%r/(size allcs)%r.
 
 require BigPr.
 clone import BigPr as BP with type ct  <- ct,
-                              type pt  <- pt,
-                              type rt  <- rt * rt,
+                              type pt  <- pt * auxt,
+                              type rt  <- (rt * irt) * (rt * irt),
                               op    d  <- d,
                               op allcs <- allcs.
 
 module type Adv = {
-  proc init(p : pt) : irt
+  proc init(p : pt, aux : auxt) : irt
   proc run(i : irt, c : ct)  : rt
 }.
 
 
 
 module InitRun2(A : Adv) = {
-  proc run(a : pt) = {
+  proc run(a : pt, aux : auxt) = {
     var i, c1, c2, r1, r2;
-    i <- A.init(a);
+    i <- A.init(a,aux);
     
     c1 <$ d;
     r1 <- A.run(i,c1);
@@ -43,20 +43,20 @@ module InitRun2(A : Adv) = {
     c2 <$ d;
     r2 <- A.run(i,c2);
 
-    return ((c1,r1),(c2,r2));
+    return ((c1,(r1,i)),(c2,(r2,i)));
   }
 }.
 
 
 module InitRun1(A : Adv) = {
-  proc run(a : pt) = {
+  proc run(a : pt, aux : auxt) = {
     var i, c1, r1;
-    i <- A.init(a);
+    i <- A.init(a,aux);
     
     c1 <$ d;
     r1 <- A.run(i,c1);
 
-    return (c1,r1);
+    return (c1,(r1,i));
   }
 }.
 
@@ -67,27 +67,27 @@ declare module A : Adv.
 axiom A_ll : islossless A.run.
 
 local module C2 : Comp = {
-  proc rest(p : pt, c1c2 : ct * ct) : rt * rt = {
+  proc rest(p : pt * auxt, c1c2 : ct * ct) : (rt * irt) * (rt * irt) = {
     var r1, r2,i;
     i  <@ A.init(p);
     r1 <@ A.run(i,c1c2.`1);
     r2 <@ A.run(i,c1c2.`2);
-    return (r1,r2);
+    return ((r1,i),(r2,i));
   }
 }.
 
 
 local module C1 = {
-  proc rest(p : pt, c1 : ct) : rt = {
+  proc rest(p : pt * auxt, c1 : ct) : rt * irt = {
     var r1,i;
     i  <@ A.init(p);
     r1 <@ A.run(i,c1);
-    return r1;
+    return (r1,i);
   }
 }.
 
 local module X1 = {
-  proc run(p : pt) = {
+  proc run(p : pt * auxt) = {
     var c,r;
     c <$ d;
     r <- C1.rest(p,c);
@@ -98,39 +98,41 @@ local module X1 = {
 
 (* averging  *)
 local lemma x0 &m M p : 
-  big predT (fun (c : ct) => mu1 d c * Pr[C1.rest(p, c) @ &m : M (c, res)]) allcs =
-     Pr[X1.run(p) @ &m : M (res.`1, res.`2)].
+  big predT (fun (c : ct) => mu1 d c * Pr[C1.rest(p, c) @ &m : M p (c, res)]) allcs =
+     Pr[X1.run(p) @ &m : M p (res.`1, res.`2)].
 admitted.
 
 
 (* c1c2 <$ d * d ~ c1 <$ d ; c2 <$ d  *)
 local lemma x1 &m M p: 
-   Pr[X(C2).run(p) @ &m : M res] = Pr[Xseq(C2).run(p) @ &m : M res].
+   Pr[X(C2).run(p) @ &m : M p res] = Pr[Xseq(C2).run(p) @ &m : M p res].
 admitted.
+
+
    
 (* sum binding  *)
 local lemma x2 &m M p:
-  Pr[X1.run(p) @ &m : M (res.`1, res.`2)] ^ 2 <=
-  Pr[Xseq(C2).run(p) @ &m : M (res.`1.`1, res.`2.`1) /\ M (res.`1.`2, res.`2.`2)].
+  Pr[X1.run(p) @ &m : M p (res.`1, res.`2)] ^ 2 <=
+  Pr[Xseq(C2).run(p) @ &m : M p (res.`1.`1, res.`2.`1) /\ M p (res.`1.`2, res.`2.`2)].
 admitted.
    
 
 local lemma avr_lemma_6_app &m M p : 
-  Pr[ Xseq(C2).run(p) @ &m  : res.`1.`1 <> res.`1.`2 /\ M res ] 
-     = Pr[ Xseq(C2).run(p) @ &m  : M res ] 
+  Pr[ Xseq(C2).run(p) @ &m  : res.`1.`1 <> res.`1.`2 /\ M p res ] 
+     = Pr[ Xseq(C2).run(p) @ &m  : M p res ] 
      - big (fun r => fst r = snd r)  (fun (c1c2 : ct * ct) => 
                   ((mu1 d c1c2.`1) * (mu1 d c1c2.`2)) * 
-                   Pr[ C2.rest(p,c1c2) @ &m :  M (c1c2,res) ]) 
+                   Pr[ C2.rest(p,c1c2) @ &m :  M p (c1c2,res) ]) 
                    (cartprod2 allcs).
-rewrite -  (x1 &m (fun (r :  (ct * ct) * (rt * rt)) => r.`1.`1 <> r.`1.`2 /\ M r)).
-rewrite (avr_lemma_6 C2 &m M p).
+rewrite -  (x1 &m (fun p (r :  (ct * ct) * ((rt * irt) * (rt * irt))) => r.`1.`1 <> r.`1.`2 /\ M p r)).
+rewrite (avr_lemma_6 C2 &m (M p) p).
 rewrite - x1. auto.
 qed.
 
 
 local lemma avr_lemma_7_app &m M p c: 
- Pr[ C2.rest(p,(c,c)) @ &m :  M (c, res.`1) /\ M (c, res.`2) ]
-  <= Pr[ C1.rest(p,c) @ &m :  M (c, res) ].
+ Pr[ C2.rest(p,(c,c)) @ &m :  M p (c, res.`1) /\ M p (c, res.`2) ]
+  <= Pr[ C1.rest(p,c) @ &m :  M p (c, res) ].
 byequiv.
 proc.
 seq 2 2 : (={glob A,i,r1}).
@@ -141,27 +143,27 @@ qed.
 
 
 local lemma avr_lemma_8_app &m M p : 
-  Pr[ Xseq(C2).run(p) @ &m  : res.`1.`1 <> res.`1.`2 /\ M (res.`1.`1, res.`2.`1) /\ M (res.`1.`2, res.`2.`2) ] 
+  Pr[ Xseq(C2).run(p) @ &m  : res.`1.`1 <> res.`1.`2 /\ M p (res.`1.`1, res.`2.`1) /\ M p (res.`1.`2, res.`2.`2) ] 
 
-     >= Pr[ Xseq(C2).run(p) @ &m  : M (res.`1.`1, res.`2.`1) /\ M (res.`1.`2, res.`2.`2)  ] 
+     >= Pr[ Xseq(C2).run(p) @ &m  : M p (res.`1.`1, res.`2.`1) /\ M p (res.`1.`2, res.`2.`2)  ] 
      - big (fun r => fst r = snd r)  (fun (c1c2 : ct * ct) => 
                   ((mu1 d c1c2.`1) * (mu1 d c1c2.`2)) * 
-                   Pr[ C1.rest(p,c1c2.`1) @ &m :  M (c1c2.`1, res) ]) 
+                   Pr[ C1.rest(p,c1c2.`1) @ &m :  M p (c1c2.`1, res) ]) 
                    (cartprod2 allcs).
-rewrite (avr_lemma_6_app &m (fun (r :  (ct * ct) * (rt * rt)) =>   M (r.`1.`1, r.`2.`1) /\ M (r.`1.`2, r.`2.`2))).
+rewrite (avr_lemma_6_app &m (fun p (r :  (ct * ct) * ((rt * irt) * (rt * irt))) =>   M p (r.`1.`1, r.`2.`1) /\ M p (r.`1.`2, r.`2.`2))).
 simplify.
 have f2 :  big (fun (r : ct * ct) => r.`1 = r.`2)
   (fun (c1c2 : ct * ct) =>
      mu1 d c1c2.`1 * mu1 d c1c2.`2 *
-     Pr[C2.rest(p, c1c2) @ &m : M (c1c2.`1, res.`1) /\ M (c1c2.`2, res.`2)])
+     Pr[C2.rest(p, c1c2) @ &m : M p (c1c2.`1, res.`1) /\ M p (c1c2.`2, res.`2)])
   (cartprod2 allcs) <= 
   big (fun (r : ct * ct) => r.`1 = r.`2)
   (fun (c1c2 : ct * ct) =>
      mu1 d c1c2.`1 * mu1 d c1c2.`2 *
-     Pr[C1.rest(p, c1c2.`1) @ &m : M (c1c2.`1, res)]) (cartprod2 allcs).
+     Pr[C1.rest(p, c1c2.`1) @ &m : M p (c1c2.`1, res)]) (cartprod2 allcs).
 apply ler_sum. progress. 
-   have : Pr[C2.rest(p, a) @ &m : M (a.`1, res.`1) /\ M (a.`2, res.`2)] <=
-            Pr[C1.rest(p, a.`1) @ &m : M (a.`1, res)].
+   have : Pr[C2.rest(p, a) @ &m : M p (a.`1, res.`1) /\ M p (a.`2, res.`2)] <=
+            Pr[C1.rest(p, a.`1) @ &m : M p (a.`1, res)].
     rewrite H.
       have ->: a = (a.`1,a.`1).  smt. simplify.
       apply (avr_lemma_7_app &m M p ). 
@@ -176,39 +178,39 @@ qed.
 local lemma avr_lemma_9_app &m M p : 
      big (fun r => fst r = snd r)  (fun (c1c2 : ct * ct) => 
                   ((mu1 d c1c2.`1) * (mu1 d c1c2.`2)) * 
-                    Pr[ C1.rest(p,c1c2.`1) @ &m :  M (c1c2.`1, res) ]) 
+                    Pr[ C1.rest(p,c1c2.`1) @ &m :  M p (c1c2.`1, res) ]) 
                     (cartprod2 allcs)
-     = (1%r/(size allcs)%r) * Pr[ X1.run(p) @ &m :  M (res.`1, res.`2) ].
+     = (1%r/(size allcs)%r) * Pr[ X1.run(p) @ &m :  M p (res.`1, res.`2) ].
 have ->: big (fun r => fst r = snd r)  (fun (c1c2 : ct * ct) => 
                   ((mu1 d c1c2.`1) * (mu1 d c1c2.`2)) * 
-                   Pr[ C1.rest(p,c1c2.`1) @ &m :  M (c1c2.`1, res) ]) 
+                   Pr[ C1.rest(p,c1c2.`1) @ &m :  M p (c1c2.`1, res) ]) 
                    (cartprod2 allcs)
       = big (fun r => fst r = snd r)  (fun (c1c2 : ct * ct) => 
                   (1%r/(size allcs)%r) * ((mu1 d c1c2.`1) * 
-                   Pr[ C1.rest(p,c1c2.`1) @ &m :  M (c1c2.`1, res) ])) 
+                   Pr[ C1.rest(p,c1c2.`1) @ &m :  M p (c1c2.`1, res) ])) 
                    (cartprod2 allcs).
 apply eq_big. auto. 
 progress.
 rewrite ss. rewrite ss. simplify. auto. simplify. 
 have ->: big (fun (r : ct * ct) => r.`1 = r.`2)
   (fun (c1c2 : ct * ct) =>
-     (1%r/(size allcs)%r) * (mu1 d c1c2.`1 * Pr[C1.rest(p, c1c2.`1) @ &m : M (c1c2.`1, res)]))
+     (1%r/(size allcs)%r) * (mu1 d c1c2.`1 * Pr[C1.rest(p, c1c2.`1) @ &m : M p (c1c2.`1, res)]))
   (cartprod2 allcs)
  = (1%r/(size allcs)%r) * big (fun (r : ct * ct) => r.`1 = r.`2)
   (fun (c1c2 : ct * ct) =>
-      (mu1 d c1c2.`1 * Pr[C1.rest(p, c1c2.`1) @ &m : M (c1c2.`1, res)]))
+      (mu1 d c1c2.`1 * Pr[C1.rest(p, c1c2.`1) @ &m : M p (c1c2.`1, res)]))
   (cartprod2 allcs).
 rewrite mulr_sumr. auto.
 auto.
 have ->: big (fun (r : ct * ct) => r.`1 = r.`2)
   (fun (c1c2 : ct * ct) =>
-     mu1 d c1c2.`1 * Pr[C1.rest(p, c1c2.`1) @ &m : M (c1c2.`1, res)])
+     mu1 d c1c2.`1 * Pr[C1.rest(p, c1c2.`1) @ &m : M p (c1c2.`1, res)])
   (cartprod2 allcs)
    = big predT
       (fun (c : ct) =>
-         mu1 d c * Pr[C1.rest(p, c) @ &m : M (c, res)])
+         mu1 d c * Pr[C1.rest(p, c) @ &m : M p (c, res)])
           allcs.
-have ->: big predT (fun (c : ct) => mu1 d c * Pr[C1.rest(p, c) @ &m : M (c, res)]) allcs = big predT (fun (c : ct) => mu1 d c * Pr[C1.rest(p, c) @ &m : M (c, res)]) 
+have ->: big predT (fun (c : ct) => mu1 d c * Pr[C1.rest(p, c) @ &m : M p (c, res)]) allcs = big predT (fun (c : ct) => mu1 d c * Pr[C1.rest(p, c) @ &m : M p (c, res)]) 
     (map fst (filter (fun x => fst x = snd x) (cartprod2 allcs))). rewrite cart2_diag_unzip1. smt. auto.
 rewrite big_mapT. 
 rewrite - big_filter. rewrite  /(\o). auto.
@@ -217,9 +219,9 @@ qed.
 
 
 local lemma avr_lemma_10_app &m M p : 
-  Pr[ Xseq(C2).run(p) @ &m  : res.`1.`1 <> res.`1.`2 /\ M (res.`1.`1, res.`2.`1) /\ M (res.`1.`2, res.`2.`2) ] >= 
-  Pr[ Xseq(C2).run(p) @ &m  : M (res.`1.`1, res.`2.`1) /\ M (res.`1.`2, res.`2.`2)  ] 
-   - (1%r/(size allcs)%r) * Pr[ X1.run(p) @ &m :  M (res.`1, res.`2) ].
+  Pr[ Xseq(C2).run(p) @ &m  : res.`1.`1 <> res.`1.`2 /\ M p (res.`1.`1, res.`2.`1) /\ M p (res.`1.`2, res.`2.`2) ] >= 
+  Pr[ Xseq(C2).run(p) @ &m  : M p (res.`1.`1, res.`2.`1) /\ M p (res.`1.`2, res.`2.`2)  ] 
+   - (1%r/(size allcs)%r) * Pr[ X1.run(p) @ &m :  M p (res.`1, res.`2) ].
 rewrite - avr_lemma_9_app.
 apply avr_lemma_8_app.
 qed.
@@ -227,15 +229,15 @@ qed.
 
 local lemma avr_lemma_11_app &m M p : 
    Pr[ Xseq(C2).run(p) @ &m  : res.`1.`1 <> res.`1.`2 
-            /\ M (res.`1.`1, res.`2.`1) /\ M (res.`1.`2, res.`2.`2) ] 
-       >= Pr[ X1.run(p) @ &m :  M (res.`1, res.`2) ] ^2
-          - (1%r/(size allcs)%r) * Pr[ X1.run(p) @ &m :  M (res.`1, res.`2) ].
-apply (ler_trans (Pr[ Xseq(C2).run(p) @ &m  : M (res.`1.`1, res.`2.`1) 
-                                             /\ M (res.`1.`2, res.`2.`2)  ] 
-   - (1%r/(size allcs)%r) * Pr[ X1.run(p) @ &m :  M (res.`1, res.`2) ])). 
-have ff : Pr[X1.run(p) @ &m : M (res.`1, res.`2)] ^ 2
-     <= Pr[Xseq(C2).run(p) @ &m : M (res.`1.`1, res.`2.`1) 
-                                     /\ M (res.`1.`2, res.`2.`2)].
+            /\ M p (res.`1.`1, res.`2.`1) /\ M p (res.`1.`2, res.`2.`2) ] 
+       >= Pr[ X1.run(p) @ &m :  M p (res.`1, res.`2) ] ^2
+          - (1%r/(size allcs)%r) * Pr[ X1.run(p) @ &m :  M p (res.`1, res.`2) ].
+apply (ler_trans (Pr[ Xseq(C2).run(p) @ &m  : M p (res.`1.`1, res.`2.`1) 
+                                             /\ M p (res.`1.`2, res.`2.`2)  ] 
+   - (1%r/(size allcs)%r) * Pr[ X1.run(p) @ &m :  M p (res.`1, res.`2) ])). 
+have ff : Pr[X1.run(p) @ &m : M p (res.`1, res.`2)] ^ 2
+     <= Pr[Xseq(C2).run(p) @ &m : M p (res.`1.`1, res.`2.`1) 
+                                     /\ M p (res.`1.`2, res.`2.`2)].
 apply x2.
 smt. 
 apply (avr_lemma_10_app &m M p).
@@ -244,14 +246,14 @@ qed.
 
 lemma final_eq &m M p : 
    Pr[ InitRun2(A).run(p) @ &m 
-          : res.`1.`1 <> res.`2.`1 /\ M res.`1 /\ M res.`2 ] 
-  >= Pr[ InitRun1(A).run(p) @ &m  :  M res ]^2
-          - (1%r/(size allcs)%r) * Pr[ InitRun1(A).run(p) @ &m  :  M res ].
+          : res.`1.`1 <> res.`2.`1 /\ M p res.`1 /\ M p res.`2 ] 
+  >= Pr[ InitRun1(A).run(p) @ &m  :  M p res ]^2
+          - (1%r/(size allcs)%r) * Pr[ InitRun1(A).run(p) @ &m  :  M p res ].
 proof.
  have <-: Pr[ Xseq(C2).run(p) @ &m  : res.`1.`1 <> res.`1.`2 
-            /\ M (res.`1.`1, res.`2.`1) /\ M (res.`1.`2, res.`2.`2) ] 
+            /\ M p (res.`1.`1, res.`2.`1) /\ M p (res.`1.`2, res.`2.`2) ] 
     = Pr[ InitRun2(A).run(p) @ &m 
-          : res.`1.`1 <> res.`2.`1 /\ M res.`1 /\ M res.`2 ].
+          : res.`1.`1 <> res.`2.`1 /\ M p res.`1 /\ M p res.`2 ].
 byequiv. proc.  simplify.
 swap {2} 2 -1.
 swap {2} 4 -2.
@@ -261,48 +263,45 @@ call (_:true).
 call (_:true). wp.  simplify.
 rnd. rnd.
 skip. progress. auto.  auto.
- have <-: Pr[ X1.run(p) @ &m :  M (res.`1, res.`2) ] 
-    = Pr[ InitRun1(A).run(p) @ &m : M res ].
+ have <-: Pr[ X1.run(p) @ &m :  M p (res.`1, res.`2) ] 
+    = Pr[ InitRun1(A).run(p) @ &m : M p res ].
 byequiv. proc. inline*. swap {2} 2 -1. wp. 
 simplify.   call (_:true).  call (_:true). wp. rnd. 
-skip. progress. auto.  auto.
+skip. progress. auto.  auto. 
 apply avr_lemma_11_app.
 qed.
 
 
 lemma final_eq_step1 &m AccRun SuccExtr p negl : 
    Pr[ InitRun2(A).run(p) @ &m 
-          : res.`1.`1 <> res.`2.`1 /\ AccRun res.`1 /\ AccRun res.`2
-   /\ !SuccExtr res.`1 res.`2 ] <= negl
-
+          : res.`1.`1 <> res.`2.`1 /\ AccRun p res.`1 /\ AccRun p res.`2
+   /\ !SuccExtr p res.`1 res.`2 ] <= negl
   => 
    Pr[ InitRun2(A).run(p) @ &m : res.`1.`1 <> res.`2.`1 
-            /\ AccRun res.`1 /\ AccRun res.`2 /\ SuccExtr res.`1 res.`2 ] 
-
-    >= (Pr[ InitRun1(A).run(p) @ &m  :  AccRun res ]^2
-         - (1%r/(size allcs)%r) * Pr[ InitRun1(A).run(p) @ &m  :  AccRun res ])
-
+            /\ AccRun p res.`1 /\ AccRun p res.`2 /\ SuccExtr p res.`1 res.`2 ] 
+    >= (Pr[ InitRun1(A).run(p) @ &m  :  AccRun p res ]^2
+         - (1%r/(size allcs)%r) * Pr[ InitRun1(A).run(p) @ &m  :  AccRun p res ])
         - negl.
 progress.
-have : Pr[InitRun1(A).run(p) @ &m : AccRun res] ^ 2 -
-  Pr[InitRun1(A).run(p) @ &m : AccRun res] / (size allcs)%r <=
+have : Pr[InitRun1(A).run(p) @ &m : AccRun p res] ^ 2 -
+  Pr[InitRun1(A).run(p) @ &m : AccRun p res] / (size allcs)%r <=
    Pr[InitRun2(A).run(p) @ &m : res.`1.`1 <> res.`2.`1 /\
-       AccRun res.`1 /\ AccRun res.`2 /\ SuccExtr res.`1 res.`2] + negl.
+       AccRun p res.`1 /\ AccRun p res.`2 /\ SuccExtr p res.`1 res.`2] + negl.
   apply (ler_trans    Pr[ InitRun2(A).run(p) @ &m 
-          : res.`1.`1 <> res.`2.`1 /\ AccRun res.`1 /\ AccRun res.`2 ] ).
+          : res.`1.`1 <> res.`2.`1 /\ AccRun p res.`1 /\ AccRun p res.`2 ] ).
   apply final_eq.  
-rewrite Pr[mu_split SuccExtr res.`1 res.`2]. 
+rewrite Pr[mu_split SuccExtr p res.`1 res.`2]. 
 have ->: Pr[InitRun2(A).run(p) @ &m :
-   (res.`1.`1 <> res.`2.`1 /\ AccRun res.`1 /\ AccRun res.`2) /\
-   SuccExtr res.`1 res.`2] = Pr[InitRun2(A).run(p) @ &m :
-   res.`1.`1 <> res.`2.`1 /\ AccRun res.`1 /\ AccRun res.`2 /\
-   SuccExtr res.`1 res.`2].
+   (res.`1.`1 <> res.`2.`1 /\ AccRun p res.`1 /\ AccRun p res.`2) /\
+   SuccExtr p res.`1 res.`2] = Pr[InitRun2(A).run(p) @ &m :
+   res.`1.`1 <> res.`2.`1 /\ AccRun p res.`1 /\ AccRun p res.`2 /\
+   SuccExtr p res.`1 res.`2].
 rewrite Pr[mu_eq]. smt. auto.
 have ->: Pr[InitRun2(A).run(p) @ &m :
-   (res.`1.`1 <> res.`2.`1 /\ AccRun res.`1 /\ AccRun res.`2) /\
-   !SuccExtr res.`1 res.`2] = Pr[InitRun2(A).run(p) @ &m :
-   res.`1.`1 <> res.`2.`1 /\ AccRun res.`1 /\ AccRun res.`2 /\
-   !SuccExtr res.`1 res.`2].
+   (res.`1.`1 <> res.`2.`1 /\ AccRun p res.`1 /\ AccRun p res.`2) /\
+   !SuccExtr p res.`1 res.`2] = Pr[InitRun2(A).run(p) @ &m :
+   res.`1.`1 <> res.`2.`1 /\ AccRun p res.`1 /\ AccRun p res.`2 /\
+   !SuccExtr p res.`1 res.`2].
 rewrite Pr[mu_eq]. smt. auto.
 smt.
 smt.
@@ -322,44 +321,40 @@ smt. qed.
 
 lemma final_eq_step2 &m AccRun SuccExtr p negl : 
    Pr[ InitRun2(A).run(p) @ &m 
-          : res.`1.`1 <> res.`2.`1 /\ AccRun res.`1 /\ AccRun res.`2
-   /\ !SuccExtr res.`1 res.`2 ] <= negl
-
+          : res.`1.`1 <> res.`2.`1 /\ AccRun p res.`1 /\ AccRun p res.`2
+   /\ !SuccExtr p res.`1 res.`2 ] <= negl
  => Pr[ InitRun2(A).run(p) @ &m 
-          :  SuccExtr res.`1 res.`2 ] = 0%r   
-
- => Pr[ InitRun1(A).run(p) @ &m  :  AccRun res ]
+          :  SuccExtr p res.`1 res.`2 ] = 0%r   
+ => Pr[ InitRun1(A).run(p) @ &m  :  AccRun p res ]
    <=  sqrt (negl + 1%r/(size allcs)%r).
-
-
 proof.  progress.
 have f2 :     Pr[InitRun2(A).run(p) @ &m :
        res.`1.`1 <> res.`2.`1 /\
-  AccRun res.`1 /\ AccRun res.`2 /\ SuccExtr res.`1 res.`2] = 0%r.
+  AccRun p res.`1 /\ AccRun p res.`2 /\ SuccExtr p res.`1 res.`2] = 0%r.
   have ff2: Pr[InitRun2(A).run(p) @ &m :
        res.`1.`1 <> res.`2.`1 /\
-  AccRun res.`1 /\ AccRun res.`2 /\ SuccExtr res.`1 res.`2]
+  AccRun p res.`1 /\ AccRun p res.`2 /\ SuccExtr p res.`1 res.`2]
    <= 0%r. rewrite - H0.
    rewrite Pr[mu_sub]. smt. auto. 
   smt.
 have f1 :    0%r 
-    >= (Pr[ InitRun1(A).run(p) @ &m  :  AccRun res ]^2
-         - (1%r/(size allcs)%r) * Pr[ InitRun1(A).run(p) @ &m  :  AccRun res ])
+    >= (Pr[ InitRun1(A).run(p) @ &m  :  AccRun p res ]^2
+         - (1%r/(size allcs)%r) * Pr[ InitRun1(A).run(p) @ &m  :  AccRun p res ])
     - negl.
 rewrite - f2.
 apply (final_eq_step1 &m). assumption.
 clear f2. clear H.
-have f3 : Pr[InitRun1(A).run(p) @ &m : AccRun res] ^ 2 
-     <= 1%r / (size allcs)%r * Pr[InitRun1(A).run(p) @ &m : AccRun res] + negl.
+have f3 : Pr[InitRun1(A).run(p) @ &m : AccRun p res] ^ 2 
+     <= 1%r / (size allcs)%r * Pr[InitRun1(A).run(p) @ &m : AccRun p res] + negl.
 smt.
 clear f1.
 clear H0.
-have : Pr[InitRun1(A).run(p) @ &m : AccRun res] <=
-    sqrt (1%r / (size allcs)%r * Pr[InitRun1(A).run(p) @ &m : AccRun res] + negl).
+have : Pr[InitRun1(A).run(p) @ &m : AccRun p res] <=
+    sqrt (1%r / (size allcs)%r * Pr[InitRun1(A).run(p) @ &m : AccRun p res] + negl).
 apply qqq2. auto.
 clear f3. simplify.
 move => f4.
-apply (ler_trans (sqrt (Pr[InitRun1(A).run(p) @ &m : AccRun res] / (size allcs)%r + negl))).
+apply (ler_trans (sqrt (Pr[InitRun1(A).run(p) @ &m : AccRun p res] / (size allcs)%r + negl))).
 auto.
 apply qqq1. smt.
 qed.
