HC/PoK.ec
@@ -1,0 +1,106 @@
+pragma Goals:printall.
+require import AllCore DBool Bool List Distr Int Aux DJoin.
+require import Aux Permutation Basics.
+
+
+clone import PoK.
+clone import ComputationalPoK.
+
+
+
+
+
+
+
+require Generic_KE.
+
+clone import Generic_KE as GKE with type pt <- hc_prob,
+                                    type auxt <- auxiliary_input,
+                                    type irt <- hc_com,
+                                    type ct <- bool,
+                                    type rt <- hc_resp,
+                                    op d <- {0,1},
+                                    op allcs <- [false; true].
+
+
+require import SpecialSoundness.
+
+(* move to Generic_Defs?  *)
+module HC_SpecialSoundnessAdversary(P : MaliciousProver) : SpecialSoundnessAdversary = {
+  proc attack(p : hc_prob, aux : auxiliary_input) : transcript * transcript = {
+    var i,c1,c2,r1,r2;
+    i <@ P.commitment(p, aux);
+
+    c1 <$ {0,1};
+    r1 <@ P.response(c1);
+
+    c2 <$ {0,1};
+    r2 <@ P.response(c2);
+    return ((i,c1,r1), (i,c2,r2));
+  }
+}.
+
+module (Extractor : Extractor)(P : MaliciousProver) = {  
+  module SA = HC_SpecialSoundnessAdversary(P)
+
+  proc extract(p : hc_prob, aux : auxiliary_input) : hc_wit = {
+    var i,j,c1,c2,r1,r2,t1,t2;
+    
+    (t1,t2) <@ SA.attack(p, aux);
+    (i,c1,r1) <- t1;
+    (j,c2,r2) <- t2;
+    
+    return my_extract p i r1 r2;
+ }
+}.
+
+section.
+declare module P : MaliciousProver.
+
+
+op ss : hc_prob.
+op auxx : auxiliary_input.
+
+clone import SSB as SSB with op ss <- ss,
+                             op auxx <- auxx.
+
+local module A : Adv = {
+  proc init (p : hc_prob, aux : auxiliary_input) : hc_com = {
+    var i : hc_com;
+    i <@ P.commitment(p,aux);
+    return i;
+ }
+
+ proc run(hcm : hc_com, hcc: bool) : hc_resp = {
+   var r;
+   r <@ P.response(hcc);
+   return r;
+ }
+}.
+
+
+local lemma ex_a_eq &m p aux : 
+ Pr[ InitRun2(A).run(p,aux) @ &m 
+          : res.`1.`1 <> res.`2.`1  /\
+  hc_verify p res.`1.`2.`2 res.`1.`1 res.`1.`2.`1  /\
+  hc_verify p res.`2.`2.`2 res.`2.`1 res.`2.`2.`1  /\
+  ! IsHC (p, special_soundness_extract p (res.`1.`2.`2, res.`1.`1, res.`1.`2.`1) 
+                                         (res.`2.`2.`2, res.`2.`1, res.`2.`2.`1)) ] 
+  = Pr[ HC_SpecialSoundnessAdversary(P).attack(p, aux) @ &m :
+             valid_transcript_pair p res.`1 res.`2 /\
+              ! IsHC (p, special_soundness_extract p res.`1 res.`2)].
+byequiv;auto.
+proc. simplify.   
+inline*. wp.  call (_:true).  wp.  rnd.  wp. call (_:true). wp.  rnd. 
+wp.  call (_:true). wp. skip. progress;smt.
+qed.
+
+
+
+local lemma ex_a_eq2 &m  : 
+  Pr[ HC_SpecialSoundnessAdversary(P).attack(ss, auxx) @ &m :
+             valid_transcript_pair ss res.`1 res.`2 /\
+              ! IsHC (ss, special_soundness_extract ss res.`1 res.`2)]
+ <= Pr[BindingExperiment(SpecialSoundnessBinder(HC_SpecialSoundnessAdversary(P))).main() @ &m : res].
+apply (computational_special_soundness_binding (HC_SpecialSoundnessAdversary(P)) &m).
+qed.
