HC/ZK.ec
@@ -1,0 +1,813 @@
+pragma Goals:printall.
+require import AllCore DBool Bool List Distr Int Aux DJoin.
+
+require import Permutation Basics.
+import DJMM.
+
+clone import ZK.
+
+module HP' : HonestProver  = {
+  var n : int 
+  var g : graph
+  var prm : permutation
+  var w : hc_wit
+  var fal : bool list      
+
+  var zpd_g, zpd_w : bool list
+  var pi_gco, pi_wco : (commitment * opening) list
+  var pi_gwco : (commitment * opening) list
+  var pi_w : hc_wit
+  
+  proc commitment(p_a : hc_prob, w_a : hc_wit) : hc_com = {   
+    (n,g) <- p_a;
+    w <- w_a;
+    prm <$ perm_d n; 
+    fal <- fap prm g;
+    pi_w <- permute_wit prm w;
+    (zpd_g, zpd_w) <- (drop n (ip (prj pi_w) fal), 
+                            take n (ip (prj pi_w) fal));
+    (pi_wco, pi_gco) <@ DJM.main1(zpd_w, zpd_g);
+    pi_gwco <-(pi (prj pi_w)) (pi_wco ++ pi_gco);
+
+    return (map fst pi_gwco);    
+  }
+    
+  proc response(b : bool) : hc_resp = {
+    return if b then Left (prm, map snd pi_gwco) 
+          else Right (pi_w, map snd pi_wco);
+ } 
+}.
+
+
+
+section.
+declare module V : MaliciousVerifier {HonestProver,HP'}.
+declare module D : ZKDistinguisher {V,HonestProver,HP'}.
+
+axiom D_run_ll : islossless D.guess.
+axiom V_summitup_ll : islossless V.summitup.
+
+
+module ZKP(P : HonestProver, V : MaliciousVerifier) = {
+  proc run(Ny : hc_prob, w : hc_wit, b : bool) = {
+    var c,r;
+    c <- P.commitment(Ny,w);
+    r <- P.response(b);
+    return (c,r);
+  }
+}.
+
+module ZKD(P : HonestProver, V : MaliciousVerifier, D : ZKDistinguisher) = {
+  proc main(Ny : hc_prob, aux: auxiliary_input, w : hc_wit) = {
+    var c,b,r,result,rb;
+    c <- P.commitment(Ny,w);
+    b <- V.challenge(Ny,c,aux);
+    r <- P.response(b);
+    result <- V.summitup(Ny,r);
+    rb <- D.guess(Ny,w,aux,result);
+    return rb;
+  }
+}.
+
+
+lemma zkp_hp'_hp (a : hc_prob * hc_wit):  IsHC a =>
+  equiv [ ZKP(HonestProver, V).run ~ ZKP(HP',V).run : (arg{2}.`1, arg{2}.`2) = a  /\ ={arg, glob V} ==> ={res} ].
+proof. move => ishc. proc.
+seq 1 1 : (={Ny, c, glob V,b} 
+    /\ HonestProver.pi_gwco{1} = HP'.pi_gwco{2}
+    /\ a = ((HP'.n, HP'.g), HP'.w){2}
+    /\ HP'.pi_w{2} = permute_wit HP'.prm{2} HP'.w{2}
+  /\ HP'.fal{2} = fap HP'.prm{2} HP'.g{2}
+  /\  (HP'.zpd_g){2} = drop HP'.n{2} (ip (prj HP'.pi_w) HP'.fal){2}
+  /\  (HP'.zpd_w){2} = take HP'.n{2} (ip (prj HP'.pi_w) HP'.fal){2}
+    /\   (pi ((prj HP'.pi_w{2})) 
+            (HP'.pi_wco ++ HP'.pi_gco)){2} = HonestProver.pi_gwco{1}
+  /\ HonestProver.w{1} = HP'.w{2}
+  /\ HonestProver.prm{1} = HP'.prm{2}
+  /\ HonestProver.g{1} = HP'.g{2}  
+  /\ HonestProver.n{1} = HP'.n{2}  
+  /\ HonestProver.fal{1} = HP'.fal{2}
+  /\ size HP'.pi_wco{2} = size HP'.w{2}
+).
+inline HonestProver.commitment HP'.commitment. wp.
+seq 6 6 : (={Ny, glob V,b} 
+  /\ HonestProver.fal{1} = HP'.fal{2}  
+    /\ a = ((HP'.n, HP'.g), HP'.w){2}
+  /\ HonestProver.g{1} = HP'.g{2}
+  /\ HonestProver.w{1} = HP'.w{2}
+  /\ HonestProver.prm{1} = HP'.prm{2}
+  /\ HonestProver.n{1} = HP'.n{2}
+  /\ ={w_a, p_a}
+  /\ HP'.fal{2} = fap HP'.prm{2} HP'.g{2}).
+wp. rnd. wp. skip. progress.  smt. sp.
+exists* HP'.pi_w{2}.
+elim*. progress.
+simplify.
+exists* HP'.zpd_w{2}, HP'.zpd_g{2}.
+elim*. progress.
+call (djm_main511 (prj pi_w_R ) (zpd_w_R, zpd_g_R) ).
+skip. progress. smt.
+have : size result_R.`1 = HP'.n{2}.
+  have : HP'.n{2} <= size (ip (prj (permute_wit HP'.prm{2} HP'.w{2}))
+            (fap HP'.prm{2} HP'.g{2})).
+rewrite /permute_wit.  
+rewrite size_ip. rewrite fap_prop2. 
+smt.
+smt. 
+smt. auto.
+seq 2 2 : (={glob V, r ,c} ).
+inline*.
+wp.  simplify. 
+skip. progress. 
+case (b{2} = true).
+move => h.  rewrite h.
+simplify. auto.
+move => h.
+have : b{2} = false.
+smt. clear h. move => h. rewrite h. simplify.
+progress.
+rewrite   ippi. 
+smt. skip. progress.
+qed.
+
+
+
+
+(* one-time simulator  *)
+module Sim1_0(V : MaliciousVerifier, D : ZKDistinguisher) = {
+  module ZKP_HP = ZKP(HonestProver,V)
+  module ZKP_HP' = ZKP(HP',V)
+  proc sinit(p_a : hc_prob) : bool * (hc_com * hc_resp) = {
+    var n, g,bb,r;
+    (n,g) <- (p_a.`1, p_a.`2);
+
+    bb <$ {0,1};
+
+    if (bb) {
+       r <- ZKP_HP.run(p_a, witness, bb);
+    }else{
+       r <- ZKP_HP'.run((n, compl_graph n), (compl_graph_cyc n), bb);
+    }
+    return (bb, r);
+  }
+
+  proc simulate(pa : hc_prob, aux : auxiliary_input, wa : hc_wit) : bool * bool  = {
+    var b',b,zryb,result, rb;
+    (b',zryb) <- sinit(pa);
+    b <- V.challenge(pa, zryb.`1, aux);
+    result <- V.summitup(pa, zryb.`2);
+    rb <- D.guess(pa, wa, aux, result); (* need to give witness to D, but here impossible, detach Sim1 and D *)
+    return (b = b', rb);
+  }
+}.
+
+
+
+local module Sim1_1(V : MaliciousVerifier) = {
+  module ZKP_HP = ZKP(HonestProver,V)
+  module ZKP_HP' = ZKP(HP',V)
+  proc sinit(p_a : hc_prob, w_a : hc_wit) = {
+    var n, g,bb,r;
+    (n,g) <- (p_a.`1, p_a.`2);
+
+    bb <$ {0,1};
+
+    if (bb) {
+       r <- ZKP_HP.run(p_a, w_a, bb);
+    }else{
+        r <- ZKP_HP'.run((n, compl_graph n), w_a, bb);
+        (* 
+Alternative:
+
+r <- aux1(n, w_a);
+ *)
+    }
+    return (bb, r);
+  }
+
+(* 
+
+(Here or in diff. module)
+proc aux1(n, w_a) = {
+g <- compl_graph n;
+    w <- w_a;
+    prm <$ perm_d n; 
+    fal <- fap prm g;
+    pi_w <- permute_wit prm w;
+    (zpd_g, zpd_w) <- (drop n (ip (prj pi_w) fal), 
+                            take n (ip (prj pi_w) fal));
+    (pi_wco, pi_gco) <@ DJM.main1(zpd_w, zpd_g);
+    pi_gwco <-(pi (prj pi_w)) (pi_wco ++ pi_gco);
+
+    return (map fst pi_gwco, Right (pi_w, map snd pi_wco));
+}
+ *)
+
+  
+  proc simulate(pa : hc_prob, aux:auxiliary_input, wa : hc_wit) : bool * bool  = {
+    var b',b,zryb,result, rb;
+    (b',zryb) <- sinit(pa,wa);
+    b <- V.challenge(pa, zryb.`1, aux);
+    result <- V.summitup(pa,zryb.`2);
+    rb <- D.guess(pa, wa, aux, result);
+    return (b = b', rb);
+  }
+
+}.
+
+(*
+
+
+
+ZKDB ~ Sim1  
+(ZKDB is like ZKD, but outputs additionally a random bit, and if this random bit is "fail", outputs a fixed value)
+(I assume Sim1, when outputting failure, outputs a fixed value)
+
+*)
+
+local lemma sim_0_1 (a : hc_prob * hc_wit):  (fst (fst a)) = size (snd a) =>
+  equiv [ Sim1_0(V,D).simulate ~ Sim1_1(V).simulate : 
+               a .`1 = arg{2}.`1 /\ a.`2 = arg{2}.`3 /\ ={arg} /\ ={glob V, glob D} ==> ={res} ].
+proof. move => sas. proc.
+inline Sim1_0(V,D).sinit.
+inline Sim1_1(V).sinit.
+sp.
+seq 1 1 : (p_a{2} = pa{2} /\ a = (pa,wa){2} /\
+  w_a{2} = wa{2} /\
+  g{2} = p_a{2}.`2 /\
+  n{2} = p_a{2}.`1 /\
+  p_a{1} = pa{1} /\
+  g{1} = p_a{1}.`2 /\
+  n{1} = p_a{1}.`1 /\ 
+  pa{1} = pa{2} /\ ={glob V, glob D,aux,wa} /\ bb{1} = bb{2}).
+rnd. skip. progress.  smt.
+if. auto. 
+call (_:true).
+call (_:true).
+wp. inline*. wp.  call (_:true).
+ wp.  rnd.  wp. rnd. wp. skip. progress.
+rewrite H. simplify. auto. 
+seq 1 1 : (={r,bb, glob V,glob D,pa,aux,wa} /\ !bb{1}).
+inline*. 
+seq  10 10 : (HP'.pi_w{1} = HP'.pi_w{2} /\ HP'.fal{1} = HP'.fal{2}
+  /\ !b0{1} /\ b0{1} = b0{2} /\ ={bb, glob V, glob D, pa, aux,wa} /\ !bb{1}
+  /\ HP'.n{1} = HP'.n{2}).
+sp. wp.
+rnd (fun (f : permutation) => compose f (mk_perm_list_fun w{2})) 
+ (fun (f : permutation) => compose f (inv (mk_perm_list_fun w{2}))).
+skip. progress.  rewrite /compose.  smt (inv_prop2). 
+rewrite /compose.  smt. rewrite /compose. smt.
+rewrite /compose. smt (inv_prop1). 
+rewrite /permute_wit /compose. 
+have ->: pa{2}.`1 = size (wa{2}). smt.
+rewrite /compl_graph_cyc.
+rewrite -  invop. 
+rewrite map_comp. auto. 
+smt (fap_prop1).
+wp.  rnd. rnd.  wp.  skip. progress.
+rewrite H. simplify. auto.
+call (_:true).
+call (_:true).
+call (_:true).
+wp. skip. progress.
+qed.
+
+
+
+local module Sim1_2(V : MaliciousVerifier) = {
+  module ZKP_HP = ZKP(HonestProver,V)
+  module ZKP_HP' = ZKP(HP',V)
+  proc sinit(p_a : hc_prob, w_a : hc_wit) = {
+    var n, g, bb, r;
+    (n,g) <- p_a;
+
+    bb <$ {0,1};
+    if (bb) {
+       r <- ZKP_HP.run(p_a, w_a, bb);
+    }else{
+       r <- ZKP_HP'.run(p_a, w_a, bb);
+    }
+    return (bb, r);
+  }
+
+  proc simulate(pa : hc_prob, aux: auxiliary_input, wa : hc_wit) : bool * bool  = {
+    var b',b,zryb,result, rb;
+    (b',zryb) <- sinit(pa,wa);
+    b <- V.challenge(pa, zryb.`1, aux);
+    result <- V.summitup(pa,zryb.`2);
+    rb <- D.guess(pa, wa, aux, result);
+    return (b = b', rb);
+  }
+}.
+
+
+
+(* hiding props  *)
+op negl, negl2 : real.
+axiom negl2_prop : 0%r <= negl2 < 1%r/4%r.
+
+
+local lemma sim_1_2 &m pa wa aux: 
+   `|Pr[ Sim1_1(V).simulate(pa,wa,aux) @ &m : res.`1 /\ res.`2 ]
+      - Pr[ Sim1_2(V).simulate(pa,wa,aux) @ &m : res.`1 /\ res.`2 ]| 
+   <= negl.
+admitted.
+
+(**
+
+Currently: AND(res) is indist. etbween Sim11, Sim12.
+
+Instead: (success, D-output) is indist. between them
+
+local lemma sim_1_2 &m pa wa pred: 
+   `|Pr[ Sim1_1(V).simulate(pa,wa) @ &m : pred res ]
+      - Pr[ Sim1_2(V).simulate(pa,wa) @ &m : pred res ]| 
+   <= negl.
+admitted.
+
+Instead: (success, result) is indist. between them (* Here: maybe not easiest *)
+
+*)
+
+
+    
+lemma  sim1ass &m pa :
+  `|Pr[Sim1_0(V,D).simulate(pa) @ &m : res.`1] -  1%r/2%r| <= negl2.
+  (* 
+Using sim_1_2, but for Sim1, Sim1_9 (but discard rb if fails)
+Instantiate with pred := fst
+Gives: |Pr[Sim1(V).simulate(pa) @ &m : res.`1] - Pr[Sim1_9 @ &m : res.`1] | <= negl2.
+The second probability is =1/2 by simple phoare analysis.
+ *)
+admitted.
+
+
+local module Sim1_3(V : MaliciousVerifier) = {
+  module ZKP_HP = ZKP(HonestProver,V)
+  module ZKP_HP' = ZKP(HP',V)
+  proc sinit(p_a : hc_prob, w_a : hc_wit) = {
+    var n, g,bb,r;
+    (n,g) <- (p_a.`1, p_a.`2);
+    bb <$ {0,1};
+    r <- ZKP_HP.run(p_a, w_a, bb);
+    return (bb, r);
+  }
+
+  proc simulate(pa : hc_prob, aux : auxiliary_input, wa : hc_wit) : bool * bool  = {
+    var b',b,zryb,result,rb;
+    (b',zryb) <- sinit(pa,wa);
+    b <- V.challenge(pa, zryb.`1, aux);
+    result <- V.summitup(pa, zryb.`2);
+    rb <@ D.guess(pa, wa, aux, result);
+    return (b = b', rb);
+  }
+}.
+
+
+local lemma sim_2_3 (a : hc_prob * hc_wit): IsHC a =>
+  equiv [ Sim1_2(V).simulate ~ Sim1_3(V).simulate : 
+               arg{1}.`1 = a.`1 /\ arg{1}.`3 = a.`2 /\ ={arg} /\ ={glob V, glob D} ==> ={res} ].
+move => ishc.
+proc.
+inline Sim1_2(V).sinit.
+inline Sim1_3(V).sinit.
+sp.
+seq 1 1 : (p_a{2} = pa{2} /\
+  w_a{2} = wa{2} /\
+  a = (pa{2},wa{2}) /\
+  g{2} = p_a{2}.`2 /\
+  n{2} = p_a{2}.`1 /\
+  p_a{1} = pa{1} /\
+  w_a{1} = wa{1} /\
+  g{1} = p_a{1}.`2 /\
+  n{1} = p_a{1}.`1 /\ (pa{1}, wa{1}) = (pa{2}, wa{2}) /\ ={glob V, glob D, aux} /\ bb{1} = bb{2}).
+rnd. skip. progress. smt.
+case (bb{1} = true).
+rcondt {1} 1. progress. sim.
+rcondf {1} 1. progress. skip. smt.
+seq 1 1 : (p_a{2} = pa{2} /\
+  w_a{2} = wa{2} /\
+  g{2} = p_a{2}.`2 /\
+  n{2} = p_a{2}.`1 /\
+  p_a{1} = pa{1} /\
+  w_a{1} = wa{1} /\
+  g{1} = p_a{1}.`2 /\
+  n{1} = p_a{1}.`1 /\ (pa{1}, wa{1}) = (pa{2}, wa{2}) /\ ={glob V, glob D, aux} /\ bb{1} = bb{2} /\ r{1} = r{2}).
+symmetry.
+call (zkp_hp'_hp a ). simplify. skip. progress.
+sim.
+qed.
+
+
+local module Sim1_4(V : MaliciousVerifier) = {
+  module ZKP_HP = ZKP(HonestProver,V)
+  proc simulate(pa : hc_prob, aux : auxiliary_input, wa : hc_wit) : bool * bool  = {
+    var b,result,r,n,g,bb,rb;
+    (n,g) <- (pa.`1, pa.`2);
+    bb <$ {0,1};
+    r <- ZKP_HP.run(pa, wa, bb);
+    b <- V.challenge(pa, r.`1, aux);
+    result <- V.summitup(pa, r.`2);
+    rb <@ D.guess(pa, wa, aux, result);
+    return (b = bb, rb);
+  }
+}.
+
+
+local lemma sim_3_4:
+  equiv [ Sim1_3(V).simulate ~ Sim1_4(V).simulate : 
+               arg{1} = arg{2} /\ ={glob V, glob D} ==> ={res} ].
+proc. sim. 
+inline*. sp. wp. rnd. wp. rnd. wp.  rnd. skip. progress.
+qed.
+
+
+local module Sim1_5(V : MaliciousVerifier) = {
+  proc simulate(pa : hc_prob, aux: auxiliary_input, wa : hc_wit) : bool * bool  = {
+    var b,result,r1,r2,n,g,bb,rb;
+    (n,g) <- (pa.`1, pa.`2);
+    bb <$ {0,1};
+    r1 <- HonestProver.commitment(pa,wa);
+    r2 <- HonestProver.response(bb);
+    b <- V.challenge(pa, r1, aux);
+    result <- V.summitup(pa,r2);
+    rb <@ D.guess(pa, wa, aux, result);
+    return (b = bb, rb);
+  }
+}.
+
+
+local lemma sim_4_5: 
+  equiv [ Sim1_4(V).simulate ~ Sim1_5(V).simulate : 
+               arg{1} = arg{2} /\ ={glob V, glob D} ==> ={res} ].
+proc. sim. 
+inline*. sp. wp. call (_:true). 
+call (_:true).  wp. rnd. wp. rnd.  wp. rnd. skip.
+progress.
+qed.
+
+
+local module Sim1_6(V : MaliciousVerifier) = {
+  proc simulate(pa : hc_prob, aux : auxiliary_input, wa : hc_wit) : bool * bool  = {
+    var b,result,r1,r2,n,g,bb,rb;
+    (n,g) <- (pa.`1, pa.`2);
+    r1 <- HonestProver.commitment(pa,wa);
+    bb <$ {0,1};
+    b <- V.challenge(pa, r1, aux);
+    r2 <- HonestProver.response(bb);
+    result <- V.summitup(pa,r2);
+    rb <@ D.guess(pa, wa, aux, result);
+    return (b = bb, rb);
+  }
+}.
+
+
+local lemma sim_5_6: 
+  equiv [ Sim1_5(V).simulate ~ Sim1_6(V).simulate : 
+               arg{1} = arg{2} /\ ={glob V, glob D} ==> ={res} ].
+proc. swap {1} 5 -1. sim. swap {2} 3 -1. sim. qed.
+
+
+local module Sim1_7(V : MaliciousVerifier) = {
+  proc simulate(pa : hc_prob, aux: auxiliary_input, wa : hc_wit) : bool * bool  = {
+    var b,result,r1,r2,n,g,bb,rb;
+    (n,g) <- (pa.`1, pa.`2);
+    r1 <- HonestProver.commitment(pa,wa);
+    bb <$ {0,1};
+    b <- V.challenge(pa, r1, aux);
+    r2 <- HonestProver.response(b);
+    result <- V.summitup(pa,r2);
+    rb <@ D.guess(pa, wa, aux, result);
+    return (b = bb, rb);
+  }
+}.
+
+
+local lemma sim_6_7: 
+  equiv [ Sim1_6(V).simulate ~ Sim1_7(V).simulate : 
+               arg{1} = arg{2} /\ ={glob V, glob D, glob HonestProver} ==> 
+   res.`1{1} /\ res.`2{1} <=>  res.`1{2} /\ res.`2{2} ].
+proc. sp. 
+seq 3 3 : (={b,bb,r1, aux, wa, pa, glob V, glob D, glob HonestProver}).
+call (_:true). rnd. simplify.
+inline*. wp.  rnd. wp.  rnd. wp.  skip. progress.
+case (b{1} <> bb{1}).
+call {1} (_:true ==> true). apply D_run_ll. 
+call {2} (_:true ==> true). apply D_run_ll. 
+call {1} (_:true ==> true). apply V_summitup_ll. 
+call {2} (_:true ==> true). apply V_summitup_ll. 
+call {1} (_:true ==> true). proc. wp. skip. auto.
+call {2} (_:true ==> true). proc. wp. skip. auto.
+skip.  smt.
+sim. 
+qed.
+
+
+local module Sim1_8(V : MaliciousVerifier) = {
+  proc simulate(pa : hc_prob, aux: auxiliary_input, wa : hc_wit) : bool * bool  = {
+    var b,result,r1,r2,n,g,bb,rb;
+    (n,g) <- (pa.`1, pa.`2);
+    r1 <- HonestProver.commitment(pa,wa);
+    b <- V.challenge(pa,r1,aux);
+    r2 <- HonestProver.response(b);
+    result <- V.summitup(pa,r2);
+    rb <@ D.guess(pa, wa, aux, result);
+    bb <$ {0,1};
+    return (bb, rb);
+  }
+}.
+
+
+local lemma sim_7_8: 
+  equiv [ Sim1_7(V).simulate ~ Sim1_8(V).simulate : 
+               arg{1} = arg{2} /\ ={glob V, glob D} ==> ={res} ].
+proc. swap {1} 3 4.
+seq 6 6 : (={rb}). sim. 
+exists* b{1}. elim*. progress.
+rnd (fun b => b ^^ !b_L).
+skip. progress. smt. smt.
+smt.
+qed.
+
+
+local module Sim1_9(V : MaliciousVerifier) = {
+  module ZKD = ZKD(HonestProver,V,D)
+  proc simulate(pa : hc_prob, aux: auxiliary_input, wa : hc_wit) : bool * bool  = {
+    var bb,rb;
+    rb <- ZKD.main(pa,aux,wa);
+    bb <$ {0,1};
+    return (bb, rb);
+  }
+}.
+
+
+local lemma sim_8_9: 
+  equiv [ Sim1_8(V).simulate ~ Sim1_9(V).simulate : 
+               arg{1} = arg{2} /\ ={glob V, glob D, glob HonestProver} ==> ={res} ].
+proc. inline*. sim.
+qed.
+
+
+local lemma sim_2_9 a: IsHC a =>
+  equiv [ Sim1_2(V).simulate ~ Sim1_9(V).simulate : 
+               a.`1 = arg{1}.`1 /\ a.`2 = arg{1}.`3 /\ arg{1} = arg{2} /\ ={glob V, glob D, glob HonestProver} ==> 
+  res.`1{1} /\ res.`2{1} <=>  res.`1{2} /\ res.`2{2} ].
+move => ishc.
+transitivity Sim1_3(V).simulate 
+(a.`1 = arg{1}.`1 /\ a.`2 = arg{1}.`3 /\ arg{1} = arg{2} /\ ={glob V, glob D, glob HonestProver} ==> 
+  res.`1{1} /\ res.`2{1} <=>  res.`1{2} /\ res.`2{2}) (arg{1} = arg{2} /\ ={glob V, glob D, glob HonestProver} ==> 
+  res.`1{1} /\ res.`2{1} <=>  res.`1{2} /\ res.`2{2}). progress. smt. smt.
+conseq (sim_2_3 a ishc). smt. auto. 
+transitivity Sim1_4(V).simulate 
+(arg{1} = arg{2} /\ ={glob V, glob D, glob HonestProver} ==> 
+  res.`1{1} /\ res.`2{1} <=>  res.`1{2} /\ res.`2{2}) (arg{1} = arg{2} /\ ={glob V, glob D, glob HonestProver} ==> 
+  res.`1{1} /\ res.`2{1} <=>  res.`1{2} /\ res.`2{2}). progress. smt. smt.
+conseq sim_3_4. auto. auto.
+transitivity Sim1_5(V).simulate 
+(arg{1} = arg{2} /\ ={glob V, glob D, glob HonestProver} ==> 
+  res.`1{1} /\ res.`2{1} <=>  res.`1{2} /\ res.`2{2}) (arg{1} = arg{2} /\ ={glob V, glob D, glob HonestProver} ==> 
+  res.`1{1} /\ res.`2{1} <=>  res.`1{2} /\ res.`2{2}). progress. smt. smt.
+conseq sim_4_5. auto. auto.
+transitivity Sim1_6(V).simulate 
+(arg{1} = arg{2} /\ ={glob V, glob D, glob HonestProver} ==> 
+  res.`1{1} /\ res.`2{1} <=>  res.`1{2} /\ res.`2{2}) (arg{1} = arg{2} /\ ={glob V, glob D, glob HonestProver} ==> 
+  res.`1{1} /\ res.`2{1} <=>  res.`1{2} /\ res.`2{2}). progress. smt. smt.
+conseq sim_5_6. auto. auto.
+transitivity Sim1_7(V).simulate 
+(arg{1} = arg{2} /\ ={glob V, glob D, glob HonestProver} ==> 
+  res.`1{1} /\ res.`2{1} <=>  res.`1{2} /\ res.`2{2}) (arg{1} = arg{2} /\ ={glob V, glob D, glob HonestProver} ==> 
+  res.`1{1} /\ res.`2{1} <=>  res.`1{2} /\ res.`2{2}). progress. smt. smt.
+conseq sim_6_7. auto. auto.
+transitivity Sim1_8(V).simulate 
+(arg{1} = arg{2} /\ ={glob V, glob D, glob HonestProver} ==> 
+  res.`1{1} /\ res.`2{1} <=>  res.`1{2} /\ res.`2{2}) (arg{1} = arg{2} /\ ={glob V, glob D, glob HonestProver} ==> 
+  res.`1{1} /\ res.`2{1} <=>  res.`1{2} /\ res.`2{2}). progress. smt. smt.
+conseq sim_7_8. auto. auto.
+conseq sim_8_9. auto.
+qed.
+
+
+local lemma sim_9_10: 
+  equiv [ Sim1_9(V).simulate ~ ZKD(HonestProver,V,D).main : 
+               arg{1} = arg{2} /\ ={glob V, glob D, glob HonestProver} 
+                  ==> res.`2{1} = res{2} ].
+proc*.  
+inline Sim1_9(V).simulate.
+wp . rnd {1}.
+simplify. sp.  sim.
+inline*. sim. wp.  skip. progress.
+qed.
+
+
+local lemma sim_9_pr1 &m pa wa aux: 
+   Pr[ Sim1_9(V).simulate(pa, aux,wa) @ &m : res.`2 ]
+   =  Pr[ Sim1_9(V).simulate(pa,aux,wa) @ &m : res.`2 /\ res.`1 ]
+   + Pr[ Sim1_9(V).simulate(pa,aux,wa) @ &m : res.`2 /\ !res.`1 ].
+proof. rewrite Pr[mu_split res.`1]. auto. 
+qed.
+
+
+local lemma sim_9_pr2 &m pa wa aux: 
+   Pr[ Sim1_9(V).simulate(pa,aux,wa) @ &m : res.`2 /\ res.`1 ]
+   = Pr[ Sim1_9(V).simulate(pa, aux, wa) @ &m : res.`2 /\ !res.`1  ].
+proof. byequiv.
+proc. seq 1 1 : (={rb}). sim. rnd (fun x => !x). 
+skip. progress. auto. auto.
+qed.
+
+
+local lemma sim_9_pr3 &m pa wa aux: 
+   Pr[ Sim1_9(V).simulate(pa,aux,wa) @ &m : res.`2 ]
+   = 2%r * Pr[ Sim1_9(V).simulate(pa,aux,wa) @ &m : res.`2 /\ res.`1  ].
+smt (sim_9_pr1 sim_9_pr2).
+qed.
+
+
+require import Pr_arg.  
+require import AllCore Distr FSet StdRing StdOrder StdBigop List.
+(*---*) import RField RealOrder Bigreal BRA.
+import BRM.
+
+
+lemma sim1_main &m pa wa aux:  IsHC (pa,wa) =>
+   `|Pr[ Sim1_0(V,D).simulate(pa,aux,wa) @ &m : res.`1 /\ res.`2 ]
+
+      / Pr[ Sim1_0(V,D).simulate(pa,aux,wa) @ &m : res.`1 ]
+
+         - Pr[ ZKD(HonestProver,V,D).main(pa,aux,wa) @ &m : res ]| 
+
+  <= 2%r * negl + 20%r * negl2.
+proof. move => ishc.
+have ->: 
+  Pr[ ZKD(HonestProver,V,D).main(pa,aux,wa) @ &m : res ]
+  = Pr[ Sim1_9(V).simulate(pa,aux,wa) @ &m : res.`2 ]. 
+ byequiv (_: arg{1} = arg{2} /\ ={glob V, glob D, glob HonestProver}  ==> _). 
+ symmetry. conseq sim_9_10. progress;auto. auto. auto. auto.
+have ->: 
+   Pr[Sim1_0(V,D).simulate(pa,aux,wa) @ &m : res.`1 /\ res.`2]
+    = Pr[ Sim1_1(V).simulate(pa,aux,wa) @ &m : res.`1 /\ res.`2 ].
+   byequiv. 
+conseq (sim_0_1 (pa,wa) _ ). smt.  simplify. smt. auto. auto.
+have h: 
+   Pr[Sim1_0(V,D).simulate(pa,aux,wa) @ &m : res.`1]
+    = Pr[ Sim1_1(V).simulate(pa,aux,wa) @ &m : res.`1].
+   byequiv. conseq (sim_0_1 (pa,wa) _). smt. auto. auto. auto.
+smt. auto. auto.
+rewrite sim_9_pr3.
+apply (ler_trans (2%r * 
+    `|Pr[Sim1_1(V).simulate(pa, aux,wa) @ &m : res.`1 /\ res.`2] -
+        Pr[Sim1_9(V).simulate(pa, aux,wa) @ &m : res.`2 /\ res.`1]| 
+           + 20%r * negl2)).
+apply main_fin. smt. smt. smt. smt (negl2_prop). 
+rewrite h. rewrite Pr[mu_sub]. auto. auto.
+apply pr_e1. smt.  
+apply sim1ass.
+apply pr_e2. smt.
+apply sim1ass.
+have ->: Pr[Sim1_9(V).simulate(pa, aux,wa) @ &m : res.`2 /\ res.`1] =
+ Pr[Sim1_2(V).simulate(pa, aux,wa) @ &m : res.`1 /\ res.`2].
+byequiv (_: (pa, aux,wa) = arg{1} /\ arg{1} = arg{2} 
+ /\ ={glob V, glob D, glob HonestProver} ==> _). 
+symmetry. conseq (sim_2_9 (pa,wa) ishc). smt. smt. auto. auto.
+smt (sim_1_2).
+qed.    
+end section.
+
+
+require OneToManyZK.
+clone import OneToManyZK as OMZK with type prob <- hc_prob, 
+                                      type wit <- hc_wit, 
+                                      type sbits <- adv_summary, 
+                                      type event <- bool, 
+                                      type auxiliary_input <- auxiliary_input,
+                                      op E <- (fun x => fst x),
+                                      op fevent <- false.
+                                      
+module Sim1(V : MaliciousVerifier) : Simulator1 = {
+  module ZKP_HP = ZKP(HonestProver,V)
+  module ZKP_HP' = ZKP(HP',V)
+  proc sinit(p_a : hc_prob) : bool * (hc_com * hc_resp) = {
+    var n, g,bb,r;
+    (n,g) <- (p_a.`1, p_a.`2);
+    bb <$ {0,1};
+    if (bb) {
+       r <- ZKP_HP.run(p_a, witness, bb);
+    }else{
+       r <- ZKP_HP'.run((n, compl_graph n), (compl_graph_cyc n), bb);
+    }
+    return (bb, r);
+  }
+
+  proc run(pa : hc_prob, aux : auxiliary_input)   = {
+    var b',b,zryb,result;
+    (b',zryb) <- sinit(pa);
+    b <- V.challenge(pa, zryb.`1, aux);
+    result <- V.summitup(pa, zryb.`2);
+    return (b = b', result);
+  }
+}.
+
+
+axiom negl2_prop : 0%r <= negl2 < 1%r/4%r.
+lemma qqq &m (p : hc_prob) (w : hc_wit) 
+ (aux : auxiliary_input) (D <: ZKDistinguisher{HP', HonestProver}) 
+     (V <: MaliciousVerifier{D, HP', HonestProver}): 
+   islossless D.guess =>
+   islossless V.summitup =>
+   IsHC (p,w) =>  
+    `|Pr[W0(Sim1(V), D).run(p, w, aux) @ &m : fst res.`2 /\ res.`1] /
+         Pr[Sim1(V).run(p,aux) @ &m : fst res] 
+              - Pr[ ZKD(HonestProver,V,D).main(p,aux,w) @ &m : res ]| <= 2%r * negl + 20%r * negl2.
+progress.
+have ->: Pr[W0(Sim1(V), D).run(p, w, aux) @ &m : fst res.`2 /\ res.`1]
+ = Pr[ Sim1_0(V,D).simulate(p,aux,w) @ &m : res.`1 /\ res.`2 ].
+progress. byequiv;auto. proc.
+call (_:true). simplify. inline   W0(Sim1(V), D).Sim1.run. sp. wp. call (_:true).
+call (_:true). simplify. call(_:true).
+sim. skip. progress. 
+have ->: Pr[Sim1(V).run(p, aux) @ &m : fst res] = 
+ Pr[ Sim1_0(V,D).simulate(p,aux,w) @ &m : res.`1 ].
+progress. byequiv (_: _ ==> res{1}.`1 = res{2}.`1);auto. proc.
+call {2} H. simplify. inline   W0(Sim1(V), D).Sim1.run. sp. wp. call (_:true).
+call (_:true). simplify. call(_:true).
+sim. skip. progress.  smt.
+
+apply (sim1_main V D H _ _ &m p w aux). assumption.
+apply negl2_prop.
+auto.
+qed.
+
+
+
+
+module  (Simulator : Simulator)(V : MaliciousVerifier)  = {
+  module M = MW.IFB.IM.W(Sim1(V))
+  proc simulate(statement : hc_prob, n : int, aux : auxiliary_input) :
+    adv_summary = {
+       var r;
+       r <@ M.whp(fst, (statement,aux),1,n,(false,witness));
+       return r.`2;
+}
+}.
+
+
+lemma hc_statistical_zk:
+        forall (V <: MaliciousVerifier{HonestProver,HP', MW.IFB.IM.W, MW.IFB.DW}) (D <: ZKDistinguisher{HP', HonestProver, MW.IFB.IM.W, V}),
+        forall stat wit ax N &m,
+        islossless V.summitup => islossless V.challenge => islossless D.guess =>
+        IsHC (stat, wit) => 
+        0 <= N =>
+        let real_prob = Pr[ZKReal(HonestProver, V, D).run(stat, wit, ax) @ &m : res] in
+        let ideal_prob = Pr[ZKIdeal(Simulator, V, D).run(stat, wit, N, ax) @ &m : res] in
+          `|real_prob - ideal_prob| <= (2%r * negl + 20%r * negl2) + 2%r * (1%r- (1%r/2%r - negl2) ) ^ N .
+simplify. progress.
+
+have ->: 
+ `|Pr[ZKReal(HonestProver, V, D).run(stat, wit, ax) @ &m : res] -
+  Pr[ZKIdeal(Simulator, V, D).run(stat, wit, N, ax) @ &m : res]|
+ = `|Pr[ZKIdeal(Simulator, V, D).run(stat, wit, N, ax) @ &m : res] - Pr[ZKReal(HonestProver, V, D).run(stat, wit, ax) @ &m : res]|. smt.
+
+have ->: Pr[ZKIdeal(Simulator, V, D).run(stat, wit, N, ax) @ &m : res]
+ = Pr[Iter(Sim1(V), D).run(false,stat,wit,ax,N,fst) @ &m : res.`1].
+byequiv (_:  E{2} = fst /\ aux{1} = aux{2} /\ n{1} = ea{2} /\ fevent{2} = false  /\
+  statement{1} = Ny{2} /\ witness{1} = w{2} /\
+    ={glob HP', glob HonestProver, glob D, glob V, glob MW.IFB.IM.W} ==> _)  ;auto. proc.
+inline Iter(Sim1(V), D).WI.run. wp.  sp. simplify.
+call (_:true).  simplify. inline Simulator(V).simulate. wp. sp.
+call (_: ={glob Sim1, glob V, glob MW.IFB.IM.W}).  sim. skip. progress.
+progress.
+
+have ->: Pr[ZKReal(HonestProver, V, D).run(stat, wit, ax) @ &m : res]
+  = Pr[ ZKD(HonestProver,V,D).main(stat,ax,wit) @ &m : res ].
+byequiv. proc. sim. auto. auto.
+print one_to_many_zk.
+apply (one_to_many_zk (Sim1(V)) D _ _ _ &m stat wit (1%r/2%r - negl2) (2%r * negl + 20%r * negl2) N
+ 
+Pr[ZKD(HonestProver, V, D).main(stat, ax, wit) @ &m : res] ax _ _ _
+) .
+proc. call H. call H0. call (_:true).  sp.  
+seq 1 : (true). rnd. auto. rnd. auto. smt. if. inline*. sp. wp. simplify. rnd. 
+conseq (_: _ ==> true). progress. apply djoinmap_weight.
+apply Com_lossless. wp. rnd. skip.
+progress. apply perm_d_lossless.
+inline*. wp. simplify. rnd. 
+conseq (_: _ ==> true). progress. 
+apply djoinmap_weight. apply Com_lossless.
+rnd.  conseq (_: _ ==> true). progress. 
+apply djoinmap_weight. apply Com_lossless.
+wp. simplify. sp. rnd. skip. progress. apply perm_d_lossless.
+hoare. rnd. skip. smt. auto. skip. auto.
+apply H1.  auto.
+apply (qqq &m stat wit ax D V). apply H1. apply H. auto. auto.
+have ->: Pr[Sim1(V).run(stat, ax) @ &m : res.`1] = 
+ Pr[Sim1_0(V,D).simulate(stat, ax, wit) @ &m : res.`1] .
+progress. byequiv (_: _ ==> res{1}.`1 = res{2}.`1);auto. proc.
+call {2} H1. simplify. inline   W0(Sim1(V), D).Sim1.run. sp. wp. call (_:true).
+call (_:true). simplify. call(_:true).
+sim. skip. progress.  smt.
+have f : `|Pr[Sim1_0(V, D).simulate(stat, ax, wit) @ &m : res.`1] - 1%r / 2%r|
+ <= negl2. 
+apply (sim1ass V D). auto. auto. apply negl2_prop. 
+smt.
+qed.
+
